ExecutionFragmentPostfix 도 일단은 작성! - 복붙이 잘 통해서 다행이야!

Nemonuri/Executions.lean
@@ -471,6 +471,182 @@ structure ExecutionFragmentPostfix (ts: TransitionSystem) where
 
 end Definition
 
+namespace ExecutionFragmentPostfix
+
+
+variable {ts: TransitionSystem} (pf: ts.ExecutionFragmentPostfix)
+
+def states : List ts.S := pf.raw.states
+
+def actions : List ts.Act := pf.raw.actions
+
+theorem actions_length_eq_states_length : pf.actions.length = pf.states.length := pf.is_valid.length_eq.symm
+
+def mk' (states : List ts.S) (actions : List ts.Act) (req: ts.IsExecutionFragmentPostfix ⟨states, actions⟩) : ts.ExecutionFragmentPostfix :=
+  ⟨⟨states, actions⟩, req⟩
+
+
+@[defeq]
+theorem mk'_eta : mk' pf.states pf.actions pf.is_valid = pf := rfl
+
+@[defeq, simp]
+theorem mk'_states {states actions req}
+  : (@ExecutionFragmentPostfix.mk' ts states actions req).states = states :=
+  rfl
+
+@[defeq, simp]
+theorem mk'_actions {states actions req}
+  : (@ExecutionFragmentPostfix.mk' ts states actions req).actions = actions :=
+  rfl
+
+@[elab_as_elim]
+def indMk'
+  {motive: ts.ExecutionFragmentPostfix → Sort _}
+  (mk': (states : List ts.S) → (actions : List ts.Act) → (req: ts.IsExecutionFragmentPostfix ⟨states, actions⟩) → motive (ExecutionFragmentPostfix.mk' states actions req))
+  (t: ts.ExecutionFragmentPostfix)
+  : motive t :=
+  mk' t.states t.actions t.is_valid |> Eq.subst t.mk'_eta
+
+def nil : ts.ExecutionFragmentPostfix := mk' [] [] (by constructor <;> simp)
+
+
+@[defeq, simp]
+theorem nil_actions_length_eq_zero : (nil : ts.ExecutionFragmentPostfix).actions.length = 0 := rfl
+
+theorem nil_eta (req: pf.actions.length = 0) : (nil : ts.ExecutionFragmentPostfix) = pf := by
+  dsimp [ExecutionFragmentPostfix.nil]
+  conv => rhs; rw [← pf.mk'_eta]
+  congr
+  · rewrite [pf.actions_length_eq_states_length] at req
+    simpa using req
+  · simpa using req
+
+
+
+def state0 (req: 0 < pf.actions.length) : ts.S := pf.states[0]'(pf.actions_length_eq_states_length ▸ req)
+
+def action0 (req: 0 < pf.actions.length) : ts.Act := pf.actions[0]'(req)
+
+def CanStepL (state0: ts.S) : Prop := (h: 0 < pf.actions.length) → (state0 ─⌞(pf.action0 h)⌟→{ts} (pf.state0 h))
+
+@[defeq]
+theorem canStepL_def {state0} : pf.CanStepL state0 = (∀ (h: 0 < pf.actions.length), (state0 ─⌞(pf.action0 h)⌟→{ts} (pf.state0 h))) := rfl
+
+@[simp]
+theorem canStepL_actions_length_eq_zero {state0} (req: pf.actions.length = 0)
+  : pf.CanStepL state0 := by
+  dsimp [canStepL_def]; intro lm1; simp [req] at lm1
+
+theorem canStepL_actions_length_pos_imp_tr {state0} (req: 0 < pf.actions.length) (h: pf.CanStepL state0)
+  : state0 ─⌞(pf.action0 req)⌟→{ts} (pf.state0 req) := by
+  dsimp [canStepL_def] at h
+  exact h req
+
+
+def stepL (state0: ts.S) (action0: ts.Act) (req: pf.CanStepL state0) : ts.ExecutionFragmentPostfix :=
+  mk' (state0 :: pf.states) (action0 :: pf.actions) (by
+    by_cases lm1: pf.actions.length = 0
+    · constructor
+      · simp [lm1]
+      · simp [lm1]
+        rewrite [pf.actions_length_eq_states_length] at lm1
+        simpa using lm1
+    · replace lm1 := Nat.pos_of_ne_zero lm1
+      replace req := pf.canStepL_actions_length_pos_imp_tr lm1 req
+      dsimp at req
+      constructor
+      · dsimp
+        intro i lm2
+        induction i with
+        | zero => dsimp; exact req
+        | succ i _ =>
+          dsimp
+          refine pf.is_valid.states_actions_valid i ?_
+          exact Nat.lt_sub_of_add_lt lm2
+      · dsimp; rw [pf.actions_length_eq_states_length] )
+
+
+theorem stepL_actions_length_pos {pf: ts.ExecutionFragmentPostfix} {state0 action0 req} : 0 < (pf.stepL state0 action0 req).actions.length := by
+  dsimp [ExecutionFragmentPostfix.stepL]
+  simp
+
+def tail : ts.ExecutionFragmentPostfix :=
+  mk' pf.states.tail pf.actions.tail (by
+    constructor
+    · simp
+      intro i lm1
+      refine pf.is_valid.states_actions_valid (i+1) ?_
+      exact Nat.add_lt_of_lt_sub lm1
+    · simp; rw [pf.actions_length_eq_states_length] )
+
+@[defeq, simp]
+theorem tail_states : pf.tail.states = pf.states.tail := rfl
+
+@[defeq, simp]
+theorem tail_actions : pf.tail.actions = pf.actions.tail := rfl
+
+
+theorem tail_canStepL (req: 0 < pf.actions.length) : pf.tail.CanStepL (pf.state0 req) := by
+  dsimp [canStepL_def, ExecutionFragmentPostfix.state0, ExecutionFragmentPostfix.action0]
+  simp [-tsub_pos_iff_lt]
+  intro lm1
+  refine pf.is_valid.states_actions_valid 0 ?_
+  exact lm1
+
+
+theorem stepL_eta (req: 0 < pf.actions.length)
+  : (stepL pf.tail (pf.state0 req) (pf.action0 req) (pf.tail_canStepL req)) = pf := by
+  dsimp [ExecutionFragmentPostfix.stepL]
+  conv => rhs; rw [← pf.mk'_eta]
+  congr
+  · dsimp [ExecutionFragmentPostfix.state0]
+    simp [List.getElem_zero_eq_head]
+  · dsimp [ExecutionFragmentPostfix.action0]
+    simp [List.getElem_zero_eq_head]
+
+@[defeq, simp]
+theorem stepL_tail {tail state0 action0 req}
+  : (@stepL ts tail state0 action0 req).tail = tail := by
+  dsimp [ExecutionFragmentPostfix.tail, ExecutionFragmentPostfix.stepL]
+  exact tail.mk'_eta
+
+@[defeq, simp]
+theorem stepL_state0 {tail state0 action0 req}
+  : (@stepL ts tail state0 action0 req).state0 stepL_actions_length_pos = state0 := by
+  dsimp [ExecutionFragmentPostfix.state0, ExecutionFragmentPostfix.stepL]
+
+@[defeq, simp]
+theorem stepL_action0 {tail state0 action0 req}
+  : (@stepL ts tail state0 action0 req).action0 stepL_actions_length_pos = action0 := by
+  dsimp [ExecutionFragmentPostfix.action0, ExecutionFragmentPostfix.stepL]
+
+@[elab_as_elim]
+def indNilStepL
+  {motive: ts.ExecutionFragmentPostfix → Sort _}
+  (nil: motive (@ExecutionFragmentPostfix.nil ts))
+  (stepL: (tail : ts.ExecutionFragmentPostfix) → (state0 : ts.S) → (action0 : ts.Act) → (req : tail.CanStepL state0) → motive (stepL tail state0 action0 req))
+  (t: ts.ExecutionFragmentPostfix)
+  : motive t :=
+  if h: t.actions.length = 0 then
+    nil |> Eq.subst (t.nil_eta h)
+  else
+    have lm1 := Nat.pos_of_ne_zero h
+    stepL t.tail (t.state0 lm1) (t.action0 lm1) (t.tail_canStepL lm1) |> Eq.subst (t.stepL_eta lm1)
+
+@[defeq, simp]
+theorem indNilStepL_nil (req: pf.actions.length = 0) {motive nil stepL}
+  : @indNilStepL ts motive nil stepL pf = (nil |> Eq.subst (pf.nil_eta req)) :=
+  rfl
+
+@[defeq, simp]
+theorem indNilStepL_stepL (req: 0 < pf.actions.length) {motive nil stepL}
+  : @indNilStepL ts motive nil stepL pf = (stepL pf.tail (pf.state0 req) (pf.action0 req) (pf.tail_canStepL req) |> Eq.subst (pf.stepL_eta req)) :=
+  rfl
+
+
+end ExecutionFragmentPostfix
+
+
 
 section Definition
 
